full chap 01

FuncAlgo/C01_Sort.lean
@@ -1,4 +1,6 @@
 
+import Mathlib.Tactic
+
 namespace InsertSort
 
 def insert (t : Nat) (l : List Nat) : List Nat :=
@@ -21,35 +23,22 @@ inductive Sorted : List Nat → Prop where
 def is_a_sorting_algorithm (f : List Nat → List Nat) : Prop :=
   ∀ l, List.Perm (f l) l ∧ Sorted (f l)
 
-theorem insert_sorted (t: Nat) (l : List Nat) (hl: Sorted l) : Sorted (insert t l) := by
-  induction l generalizing t with
-  | nil => exact Sorted.single t
-  | cons x xs ih =>
-      cases hl with
-      |single x =>
-        rw [insert]
-        by_cases htx : t ≤ x
-        .
-          rw [if_pos htx]; exact Sorted.cons t x [] htx (Sorted.single x)
-        .
-          rw [if_neg htx]; exact Sorted.cons x t [] (Nat.le_of_not_le htx) (Sorted.single t)
-      |cons _ y tl hxy htl =>
-         rw [insert]
-         by_cases htx : t ≤ x
-         . -- t ≤ x
-           rw [if_pos htx]; apply Sorted.cons t x (y :: tl) htx (Sorted.cons x y tl hxy htl)
-         . -- t > x
-           rw [if_neg htx, insert]
-           have h4 := ih t htl
-           by_cases hty : t ≤ y
-           . -- t ≤ y
-             rw [if_pos hty]
-             apply Sorted.cons x t (y :: tl) (Nat.le_of_not_le htx) _
-             apply Sorted.cons t y tl hty htl
-           . -- t > y
-             rw [if_neg hty]
-             simp [insert, if_neg hty] at h4
-             apply Sorted.cons x y (insert t tl) hxy h4
+
+theorem insert_sorted (t : Nat) (l : List Nat) (hl : Sorted l) : Sorted (insert t l) := by
+  induction hl generalizing t with
+  | nil => unfold insert; exact Sorted.single t
+  | single x =>
+      unfold insert; split_ifs with htx <;> apply Sorted.cons _ _ [] (by linarith) (Sorted.single _)
+  | cons x0 x1 lst h_x0_x1 h_x1_lst ih  =>
+      unfold insert; split_ifs with htx
+      · -- t ≤ x0
+        apply Sorted.cons t x0 (x1 :: lst) htx _
+        have h2 := ih x0; unfold insert at h2; rw [if_pos h_x0_x1] at h2
+        exact h2
+      · -- t > x0
+        have h3 := ih t; unfold insert at h3 ⊢
+        split_ifs at h3 ⊢ with htx1 <;> apply Sorted.cons x0 _ _  (by linarith) h3
+
 
 theorem sort_sorted (l : List Nat) : Sorted (sort l) := by
   induction l with
@@ -62,10 +51,8 @@ theorem insert_perm (t : Nat) (l : List Nat) : List.Perm (t :: l) (insert t l) :
   | cons x xs ih =>
       unfold insert;
       by_cases htx : t ≤ x
-      .
-        rw [if_pos htx]
-      .
-        rw [if_neg htx]
+      · rw [if_pos htx]
+      · rw [if_neg htx]
         apply List.Perm.trans (l₂ := x :: t :: xs )
           (List.Perm.swap x t xs)
           (List.Perm.cons x ih)
@@ -81,5 +68,204 @@ theorem insertion_sort_correct : is_a_sorting_algorithm sort := by
   intro lst
   apply And.intro (sort_perm lst).symm (sort_sorted lst)
 
+
+def Sorted' (lst : List Nat) : Prop := ∀ (i j iv jv: Nat),
+  i < j →
+  lst[i]? = some iv →
+  lst[j]? = some jv →
+  iv ≤ jv
+
+
+
+theorem sorted_sorted' : ∀ lst, Sorted lst → Sorted' lst := by
+  intro lst h_lst;
+  induction h_lst with
+  | nil => unfold Sorted'; intro i j iv jv hij h_iv h_jv; cases i <;> simp at h_iv
+  | single x =>
+      unfold Sorted'; intro i j iv jv hij h_iv h_jv;
+      match i, j with
+      | 0, 0 => simp at h_iv h_jv; linarith
+      | i+1, _ => simp at h_iv
+      | _, j+1 => simp at h_jv
+  | cons x y lst h_xy h_yl ih =>
+      unfold Sorted'; intro i j iv jv hij h_iv h_jv;
+      match i, j with
+      | i, 0 => simp at hij
+      | 0, 1 => simp at h_iv h_jv; linarith
+      | i+1, 1 => simp at hij
+      | 0, j+2 =>
+         simp at h_iv h_jv;
+         have h3 := ih 0 (j+1) y jv (by linarith) (by simp) (by tauto)
+         linarith
+      | i+1, j+1 => simp at h_iv h_jv; apply ih i j iv jv (by linarith) h_iv h_jv
+
+-- ---------------------------------
+
+def List_fa (lst : List Nat) (f : Nat -> Prop) : Prop :=
+  ∀ (i iv: Nat), lst[i]? = some iv -> f iv
+
+theorem list_fa_cdr : ∀ (x : Nat) (xs : List Nat) (f: Nat -> Prop),
+  List_fa (x :: xs) f -> List_fa xs f := by
+  intro x xs f h_f_x_xs i iv h_iv
+  apply h_f_x_xs (i+1) iv (by tauto)
+
+
+theorem list_fa_nil : ∀ (f : Nat -> Prop), List_fa [] f := by
+  intro f i iv h_iv
+  cases i <;> simp at h_iv
+
+theorem list_fa_cons : ∀ (f : Nat -> Prop) (x: Nat) (xs: List Nat),
+  f x -> List_fa xs f -> List_fa (x :: xs) f := by
+  intro f x xs h_fx h_fxs i iv h_iv
+  match i with
+  | 0 => simp at h_iv; rw [<- h_iv]; assumption
+  | i+1 => simp at h_iv; exact h_fxs i iv h_iv
+
+
+theorem list_fa_perm : ∀ (l1 l2 : List Nat) (f: Nat -> Prop),
+  List.Perm l1 l2 -> List_fa l1 f -> List_fa l2 f := by
+  intro l1 l2 f h_l1_l2
+  induction h_l1_l2 with
+  | nil => tauto
+  | @cons x l1 l2 h_l1_l2 ih_l1_l2 =>
+      intro h i iv h_iv
+      cases i with
+      | zero => simp at h_iv ; have h3 := h 0 iv; simp at h3; apply h3 h_iv;
+      | succ i => simp at h_iv; apply ih_l1_l2 (list_fa_cdr _ _ _ h) i iv h_iv
+  | @swap x y lst =>
+      intro h i iv h_iv;
+      match i with
+      | 0 => simp at h_iv; have h3 := h 1 iv; simp at h3; apply h3 h_iv
+      | 1 => simp at h_iv; have h3 := h 0 iv; simp at h3; apply h3 h_iv
+      | i+2 => simp at h_iv; have h3 := h (i+2) iv; simp at h3; apply h3 h_iv
+  | @trans l1 l2 l3 h_l1_l2 h_l2_l3 ih_l1_l2 ih_l2_l3 =>
+      intro h; apply ih_l2_l3 (ih_l1_l2 h)
+
+theorem sorted'_nil : Sorted' [] := by
+  unfold Sorted'; intro i j iv jv h_ij h_iv h_jv
+  match i, j with
+  | i, 0 => simp at h_ij
+  | i, j+1 => simp at h_jv
+
+theorem sorted'_single : ∀ x, Sorted' [x] := by
+  unfold Sorted'; intro x i j iv jv h_ij h_iv h_jv
+  match i, j with
+  | i, 0 => simp at h_ij
+  | i, j+1 => simp at h_jv
+
+theorem sorted'_cdr : ∀ {x xs}, Sorted' (x :: xs) → Sorted' xs := by
+  intro x xs h_x_xs i j iv jv h_ij h_iv h_jv
+  apply h_x_xs (i+1) (j+1) iv jv (by linarith) (by tauto) (by tauto)
+
+theorem sorted'_cons :
+  ∀ {x xs}, Sorted' xs → List_fa xs (fun t => x ≤ t) -> Sorted' (x :: xs) := by
+  intro x xs h_xs h_x_xs i j iv jv h_ij h_iv h_jv
+  match i, j with
+  | i, 0 => simp at h_ij
+  | 0, j+1 => simp at h_iv h_jv; rw [<- h_iv]; apply h_x_xs j jv h_jv
+  | i+1, j+1 =>
+      simp at h_iv h_jv;
+      exact h_xs i j iv jv (by linarith) (h_iv) (h_jv)
+
+theorem sorted'_cons_cons :
+  ∀ {x0 x1 xs}, x0 ≤ x1 -> Sorted' (x1 :: xs) -> Sorted' (x0 :: x1 :: xs) := by
+  intro x0 x1 xs h_x0_x1 h_x1_xs
+  apply sorted'_cons h_x1_xs _
+  intro i iv h_iv
+  match i with
+  | 0 => simp at h_iv; linarith
+  | i+1 =>
+      simp at h_iv;
+      have h2 := h_x1_xs 0 (i+1) x1 iv (by linarith) (by tauto) (by tauto)
+      linarith
+
+theorem sorted'_x0_x1_xs_sorted'_x0_xs :
+  ∀ {x0 x1 xs}, Sorted' (x0 :: x1 :: xs) → Sorted' (x0 :: xs) := by
+  intro x0 x1 xs h_x0_x1_xs
+  have h_sorted_xs := h_x0_x1_xs |> sorted'_cdr |> sorted'_cdr
+  apply sorted'_cons h_sorted_xs _; intro i iv h_iv;
+  apply h_x0_x1_xs 0 (i+2) x0 iv (by linarith) (by tauto) (by tauto)
+
+theorem sorted'_sorted : ∀ lst, Sorted' lst → Sorted lst := by
+  intro lst h_lst
+  induction lst with
+  | nil => tauto
+  | cons x xs ih =>
+      cases xs with
+      | nil => exact Sorted.single x
+      | cons x1 xs =>
+          have h_x_x1 : x ≤ x1 := h_lst 0 1 x x1 (by linarith) (by tauto) (by tauto)
+          apply Sorted.cons x x1 xs h_x_x1 (ih (sorted'_cdr h_lst))
+
+
+def elem_in_list (t : Nat) (lst : List Nat) : Prop := ∃ (i: Nat), lst[i]? = some t
+
+
+
+
+theorem elem_in_xs_elem_in_x_xs : ∀ {t x : Nat} {xs: List Nat},
+  elem_in_list t xs -> elem_in_list t (x :: xs) := by
+  intro t x xs ⟨i, hi⟩; exists (i+1)
+
+theorem elem_in_x_xs : ∀ {t x : Nat} {xs: List Nat},
+  elem_in_list t (x :: xs) -> t = x ∨ elem_in_list t xs := by
+  intro t x xs ⟨i, hi⟩
+  match i with
+  | 0 => simp at hi; rw[hi]; tauto
+  | i+1 => simp at hi; right; exists i
+
+theorem elem_in_perm : ∀ {t : Nat} {l1 l2 : List Nat},
+  List.Perm l1 l2 -> elem_in_list t l1 -> elem_in_list t l2 := by
+  intro t l1 l2 h_l1_l2
+  induction h_l1_l2 generalizing t with
+  | nil => tauto
+  | @trans l1 l2 l3 h_l12 h_l23 ih_l12 ih_l23 => intro h; exact ih_l23 (ih_l12 h)
+  | @swap  x y lst =>
+      intro ⟨i, hi⟩
+      match i with
+      | 0 => exists 1
+      | 1 => exists 0
+      | j+2 => exists (j+2)
+  | @cons x l1 l2 h_l1_l2 ih =>
+      intro h_t_x_l1
+      match (elem_in_x_xs h_t_x_l1) with
+      | Or.inl left => exists 0; simp; tauto;
+      | Or.inr right =>
+          apply elem_in_xs_elem_in_x_xs (ih right);
+
+theorem nth_error_insert : ∀ (l: List Nat) (a i iv: Nat),
+    (insert a l)[i]? = some iv →
+    a = iv ∨ ∃ (i': Nat), l[i']? = some iv := by
+    intro lst a i iv h1
+    rw [eq_comm, <- elem_in_list]
+    apply elem_in_x_xs
+    have h1 : elem_in_list iv (insert a lst) := by exists i
+    exact elem_in_perm (t := iv) (l1 := insert a lst) (l2 := a :: lst) (insert_perm a lst).symm h1
+
+theorem insert_sorted' : ∀ a lst, Sorted' lst → Sorted' (insert a lst) := by
+  intro a lst h_lst
+  induction lst generalizing a with
+  | nil => unfold insert; apply sorted'_single
+  | cons x xs ih =>
+      unfold insert
+      split_ifs with h_ax
+      · apply sorted'_cons_cons h_ax h_lst
+      · have h7 := ih a (sorted'_cdr h_lst)
+        have h8 := sorted'_cons (x := x) (xs := insert a xs) h7
+        apply h8
+        apply list_fa_perm _ _ (fun t => x ≤ t) (insert_perm a xs)
+        intro i iv h_iv
+        match i with
+        | 0 => simp at h_iv; linarith
+        | i+1 =>
+            simp at h_iv;
+            apply h_lst 0 (i+1) x iv (by linarith) (by tauto) h_iv
+
+theorem sort_sorted': ∀ l, Sorted' (sort l) := by
+  intro l
+  induction l with
+  | nil => unfold sort; exact sorted'_nil
+  | cons x xs ih =>
+      unfold sort; apply insert_sorted' x (sort xs) ih
 
 end InsertSort
